split files.

coq/theories/htmlescape.v
@@ -5,88 +5,14 @@ Require Import Ascii.
 Require Import htmlescape.listutils.
 Require Import htmlescape.assoc.
 Require Import htmlescape.ssrstr.
-
-Local Open Scope string_scope. (* enable "string-literal" and str ++ str *)
-Local Open Scope seq_scope. (* prefer seq ++ seq over str ++ str *)
-
-Definition assoc {A : eqType} {B : Type} (a : A) (al : seq (A * B)) :=
-  nosimpl (@assoc.assoc A B a al).
-
-Definition rassoc {A : Type} {B : eqType} (b : B) (al : seq (A * B)) :=
-  nosimpl (@assoc.rassoc A B b al).
-
-Definition html_escape_alist :=
-  map (fun p => (p.1, seq_of_str p.2)) [::
-  ("&"%char, "amp");
-  ("<"%char, "lt");
-  (">"%char, "gt");
-  (""""%char, "quot");
-  ("'"%char, "#39")
-].
-
-Definition html_escape_byte c :=
-  if assoc c html_escape_alist is Some p then
-    "&" ++ p.2 ++ ";"
-  else
-    [:: c].
-
-Definition html_escape s := flatten (map html_escape_byte s).
-
-Goal html_escape "abc&def<>""'" = "abc&amp;def&lt;&gt;&quot;&#39;". by []. Qed.
+Require Import htmlescape.spec.
+Require Import htmlescape.imp.
 
 Lemma html_escape_cat s1 s2 : html_escape (s1 ++ s2) = html_escape s1 ++ html_escape s2.
 Proof. by rewrite /html_escape -flatten_cat map_cat. Qed.
 
 Lemma html_escape_cons c s : html_escape (c :: s) = html_escape_byte c ++ html_escape s.
 Proof. by rewrite /html_escape /flatten. Qed.
-
-Definition html_char_entities :=
-  map (fun p => (p.1, seq_of_str p.2)) [::
-  ("&"%char, "amp");
-  ("<"%char, "lt");
-  (">"%char, "gt");
-  (""""%char, "quot");
-  ("'"%char, "apos")
-  (* ... more character entities here ... *)
-].
-
-Fixpoint html_unescape s :=
-  match s with
-  | nil => nil
-  | "&"%char :: s1 =>
-      if ci_start_with "#x" s1 is Some n1 then
-        let s2 := drop n1 s1 in
-        let (v, n2) := decode_hex_prefix s2 in
-        if n2 == 0 then "&"%char :: html_unescape s1 else
-        let s3 := drop n2 s2 in
-        if start_with ";" s3 is Some n3 then
-          (ascii_of_nat v) :: html_unescape (drop n3 s3)
-        else
-          "&"%char :: html_unescape s1
-      else if start_with "#" s1 is Some n1 then
-        let s2 := drop n1 s1 in
-        let (v, n2) := decode_decimal_prefix s2 in
-        if n2 == 0 then "&"%char :: html_unescape s1 else
-        let s3 := drop n2 s2 in
-        if start_with ";" s3 is Some n3 then
-          (ascii_of_nat v) :: html_unescape (drop n3 s3)
-        else
-          "&"%char :: html_unescape s1
-      else if sindex ";"%char s1 is Some n1 then
-        let name := take n1 s1 in
-        let s2 := drop n1 s1 in
-        if start_with ";" s2 is Some n2 then
-          let s3 := drop n2 s2 in
-          if rassoc name html_char_entities is Some (c, _) then
-            c :: html_unescape s3
-          else
-            "&"%char :: html_unescape s1
-        else
-          "&"%char :: html_unescape s1
-      else
-        "&"%char :: html_unescape s1
-  | c :: s1 => c :: html_unescape s1
-  end.
 
 Lemma html_unescape_escape s : html_unescape (html_escape s) = s.
 Proof.
@@ -108,25 +34,6 @@ Proof.
   case; first by rewrite /= IH. (* MSB of "&" *)
   by [].
 Qed.
-
-(* HTML character and text specification.
- * https://html.spec.whatwg.org/multipage/syntax.html#text-2
- * Note: Unicode is not considered.
- *)
-Inductive char_spec : ascii -> seq ascii -> Prop :=
-  | char_normal : forall c, c != "&"%char -> char_spec c [:: c]
-  | char_named : forall c entity, (c, entity) \in html_char_entities ->
-      char_spec c ("&" ++ entity ++ ";")
-  | char_dec : forall m digs, digs != nil -> decode_decimal digs = Some m ->
-      char_spec (ascii_of_nat m) ("&#" ++ digs ++ ";")
-  | char_hex : forall x m xdigs,
-      downcase_ascii x == "x"%char -> xdigs != nil -> decode_hex xdigs = Some m ->
-      char_spec (ascii_of_nat m) ("&#" ++ x :: xdigs ++ ";").
-
-Inductive text_spec : seq ascii -> seq ascii -> Prop :=
-  | text_empty : text_spec [::] [::]
-  | text_cons : forall c s raw escaped,
-      char_spec c s -> text_spec raw escaped -> text_spec (c :: raw) (s ++ escaped).
 
 Lemma html_unescape_ok raw escaped :
   text_spec raw escaped -> html_unescape escaped = raw.
@@ -209,86 +116,6 @@ Proof.
     by rewrite eq_sym.
   by apply IH.
 Qed.
-
-(* pointer to byte (unsigned char).
-  "cptr i lst" represents a pointer to i'th char in lst.
-  restriction: 0 <= i <= size lst.
-  Although a pointer with i = size lst is valid, its dereference is invalid.
-*)
-Inductive byteptr := bptr : nat -> seq ascii -> byteptr.
-
-(* accessors for Coq proof *)
-Definition i_of_bptr ptr := let: bptr i s := ptr in i.
-Definition s_of_bptr ptr := let: bptr i s := ptr in s.
-
-(* precondition: i + n <= size s
-  C: p + n *)
-Definition bptradd ptr n :=
-  let i := i_of_bptr ptr in
-  let s := s_of_bptr ptr in
-  bptr (i + n) s.
-
-(* precondition: n <= i
-  C: p - n *)
-Definition bptrsub ptr n :=
-  let i := i_of_bptr ptr in
-  let s := s_of_bptr ptr in
-  bptr (i - n) s.
-
-(* precondition: i < size s
-  C: *p *)
-Definition bptrget ptr :=
-  let i := i_of_bptr ptr in
-  let s := s_of_bptr ptr in
-  nth "000"%char s i.
-
-(* buffer implemented using Ruby String.
-  Encoding is not considiered.
-  The C type is struct rbuf { size_t len; VALUE str }.
-  "len" is used to detect the non-linear use of the string.
-  If the string is used linearly, len == RSTRING_LEN(str) is hold.
-  We assume this condition in following explanation.
- *)
-Inductive buffer := bufctr of seq ascii.
-
-(* accessor for Coq proof *)
-Definition s_of_buf buf := let: bufctr s := buf in s.
-
-(* (struct rbuf){ len + 1, rb_str_buf_cat(str, &b, 1) } *)
-Definition bufaddbyte buf b :=
-  let s := s_of_buf buf in
-  bufctr (rcons s b).
-
-(* precondition: i + n <= size s'
-  (struct rbuf){ len + n, rb_str_buf_cat(str, ptr, n) }
- *)
-Definition bufaddmem buf ptr n :=
-  let s := s_of_buf buf in
-  let i := i_of_bptr ptr in
-  let s' := s_of_bptr ptr in
-  bufctr (s ++ take n (drop i s')).
-
-(* This function will be implemented as a table in C *)
-Definition html_escape_byte_table c :=
-  if assoc c html_escape_alist is Some p then
-    let s := "&" ++ p.2 ++ ";" in
-    (bptr 0 s, size s)
-  else
-    (bptr 0 [:: c], 1).
-
-Fixpoint trec_html_escape buf ptr n :=
-  match n with
-  | 0 => buf
-  | n'.+1 =>
-      let: (escptr, escn) := html_escape_byte_table (bptrget ptr) in
-      trec_html_escape
-        (bufaddmem buf escptr escn)
-        (bptradd ptr 1)
-        n'
-  end.
-
-Definition trec_html_escape_stub s :=
-  s_of_buf (trec_html_escape (bufctr [::]) (bptr 0 s) (size s)).
 
 Definition html_escape_byte_ptr c :=
   if assoc c html_escape_alist is Some p then
@@ -383,22 +210,6 @@ Proof.
   by rewrite trec_html_escape_ok1; first rewrite drop0.
 Qed.
 
-Inductive m128 := c128 :
-  ascii -> ascii -> ascii -> ascii ->
-  ascii -> ascii -> ascii -> ascii ->
-  ascii -> ascii -> ascii -> ascii ->
-  ascii -> ascii -> ascii -> ascii -> m128.
-
-Definition seq_of_m128 m :=
-  let: c128 b0 b1 b2 b3 b4 b5 b6 b7 b8 b9 ba bb bc bd be bf := m in
-  [:: b0; b1; b2; b3; b4; b5; b6; b7; b8; b9; ba; bb; bc; bd; be; bf].
-
-Definition m128_of_seq s := c128
-  (nth "000"%char s 0) (nth "000"%char s 1) (nth "000"%char s 2) (nth "000"%char s 3)
-  (nth "000"%char s 4) (nth "000"%char s 5) (nth "000"%char s 6) (nth "000"%char s 7)
-  (nth "000"%char s 8) (nth "000"%char s 9) (nth "000"%char s 10) (nth "000"%char s 11)
-  (nth "000"%char s 12) (nth "000"%char s 13) (nth "000"%char s 14) (nth "000"%char s 15).
-
 Lemma m128_of_seq_of_m128 m : m128_of_seq (seq_of_m128 m) = m.
 Proof.
   by case: m.
@@ -473,17 +284,6 @@ Proof.
   by case: m.
 Qed.
 
-Definition m128_of_bptr ptr := m128_of_seq (drop (i_of_bptr ptr) (s_of_bptr ptr)).
-
-(* _mm_cmpestri(a, la, b, lb,
-     _SIDD_UBYTE_OPS|_SIDD_CMP_EQUAL_ANY|
-     _SIDD_POSITIVE_POLARITY|_SIDD_LEAST_SIGNIFICANT) *)
-Definition cmpestri_ubyte_eqany_ppol_lsig (a : m128) (la : nat) (b : m128) (lb : nat) :=
-  let sa := take la (seq_of_m128 a) in
-  let sb := take lb (seq_of_m128 b) in
-  let p := mem sa in
-  if has p sb then find p sb else 16.
-
 Lemma cmpestri_minn16la a la b lb : cmpestri_ubyte_eqany_ppol_lsig a la b lb =
   cmpestri_ubyte_eqany_ppol_lsig a (minn 16 la) b lb.
 Proof.
@@ -497,10 +297,6 @@ Proof.
   rewrite /cmpestri_ubyte_eqany_ppol_lsig.
   by rewrite minnC take_minn [take 16 _]take_seq_of_m128.
 Qed.
-
-Definition chars_to_escape_list := [:: "&"%char; "<"%char; ">"%char; """"%char; "'"%char].
-Definition chars_to_escape := m128_of_seq chars_to_escape_list.
-Definition num_chars_to_escape := size chars_to_escape_list.
 
 Lemma cmpestri_none a b :
   size a <= 16 -> size b <= 16 ->
@@ -569,32 +365,6 @@ Proof.
   rewrite Hif.
   by apply nth_find.
 Qed.
-
-Fixpoint sse_html_escape buf ptr m n :=
-  match n with
-  | 0 => bufaddmem buf ptr m
-  | n'.+1 =>
-      let p1 := bptradd ptr m in
-      if n <= 15 then
-        trec_html_escape (bufaddmem buf ptr m) p1 n
-      else
-        let i := cmpestri_ubyte_eqany_ppol_lsig
-            chars_to_escape num_chars_to_escape
-            (m128_of_bptr p1) 16 in
-        if 16 <= i then
-          sse_html_escape buf ptr (m + 16) (n' - 15)
-        else
-          let buf2 := bufaddmem buf ptr (m + i) in
-          let p2 := bptradd ptr (m + i) in
-          let c := bptrget p2 in
-          let p3 := bptradd p2 1 in
-          let: (escptr, escn) := html_escape_byte_table c in
-          let buf3 := bufaddmem buf2 escptr escn in
-          sse_html_escape buf3 p3 0 (n' - i)
-  end.
-
-Definition sse_html_escape_stub s :=
-  s_of_buf (sse_html_escape (bufctr [::]) (bptr 0 s) 0 (size s)).
 
 Require Import Wf_nat.
 
@@ -753,22 +523,3 @@ Proof.
   rewrite /sse_html_escape_stub.
   by rewrite sse_html_escape_ok1; first rewrite take0 drop0.
 Qed.
-
-Require Import Monomorph.monomorph.
-
-Terminate Monomorphization html_escape_byte_table.
-
-Terminate Monomorphization cmpestri_ubyte_eqany_ppol_lsig.
-Terminate Monomorphization chars_to_escape.
-Terminate Monomorphization m128_of_bptr.
-Terminate Monomorphization bptradd.
-Terminate Monomorphization bptrget.
-Terminate Monomorphization bufaddmem.
-Terminate Monomorphization addn.
-Terminate Monomorphization subn.
-Terminate Monomorphization leq.
-
-Monomorphization trec_html_escape.
-Monomorphization sse_html_escape.
-GenCFile "gen/esc.c" _trec_html_escape _sse_html_escape.
-
