coq/theories/gen.v
@@ -1,0 +1,26 @@
+From mathcomp Require Import all_ssreflect.
+Require Import String.
+Require Import Ascii.
+
+Require Import htmlescape.listutils.
+Require Import htmlescape.assoc.
+Require Import htmlescape.ssrstr.
+Require Import htmlescape.spec.
+Require Import htmlescape.imp.
+
+Require Import Monomorph.monomorph.
+
+Terminate Monomorphization html_escape_byte_table.
+Terminate Monomorphization cmpestri_ubyte_eqany_ppol_lsig.
+Terminate Monomorphization chars_to_escape.
+Terminate Monomorphization m128_of_bptr.
+Terminate Monomorphization bptradd.
+Terminate Monomorphization bptrget.
+Terminate Monomorphization bufaddmem.
+Terminate Monomorphization addn.
+Terminate Monomorphization subn.
+Terminate Monomorphization leq.
+
+Monomorphization trec_html_escape.
+Monomorphization sse_html_escape.
+GenCFile "gen/esc.c" _trec_html_escape _sse_html_escape.
