coq/theories/imp.v
@@ -1,0 +1,217 @@
+From mathcomp Require Import all_ssreflect.
+Require Import String.
+Require Import Ascii.
+
+Require Import htmlescape.listutils.
+Require Import htmlescape.assoc.
+Require Import htmlescape.ssrstr.
+
+Definition assoc {A : eqType} {B : Type} (a : A) (al : seq (A * B)) :=
+  nosimpl (@assoc.assoc A B a al).
+
+Definition rassoc {A : Type} {B : eqType} (b : B) (al : seq (A * B)) :=
+  nosimpl (@assoc.rassoc A B b al).
+
+Definition html_escape_alist :=
+  map (fun p => (p.1, seq_of_str p.2)) [::
+  ("&"%char, "amp");
+  ("<"%char, "lt");
+  (">"%char, "gt");
+  (""""%char, "quot");
+  ("'"%char, "#39")
+].
+
+Definition html_escape_byte c :=
+  if assoc c html_escape_alist is Some p then
+    "&" ++ p.2 ++ ";"
+  else
+    [:: c].
+
+Definition html_escape s := flatten (map html_escape_byte s).
+
+Goal html_escape "abc&def<>""'" = "abc&amp;def&lt;&gt;&quot;&#39;". by []. Qed.
+
+Definition html_char_entities :=
+  map (fun p => (p.1, seq_of_str p.2)) [::
+  ("&"%char, "amp");
+  ("<"%char, "lt");
+  (">"%char, "gt");
+  (""""%char, "quot");
+  ("'"%char, "apos")
+  (* ... more character entities here ... *)
+].
+
+Fixpoint html_unescape s :=
+  match s with
+  | nil => nil
+  | "&"%char :: s1 =>
+      if ci_start_with "#x" s1 is Some n1 then
+        let s2 := drop n1 s1 in
+        let (v, n2) := decode_hex_prefix s2 in
+        if n2 == 0 then "&"%char :: html_unescape s1 else
+        let s3 := drop n2 s2 in
+        if start_with ";" s3 is Some n3 then
+          (ascii_of_nat v) :: html_unescape (drop n3 s3)
+        else
+          "&"%char :: html_unescape s1
+      else if start_with "#" s1 is Some n1 then
+        let s2 := drop n1 s1 in
+        let (v, n2) := decode_decimal_prefix s2 in
+        if n2 == 0 then "&"%char :: html_unescape s1 else
+        let s3 := drop n2 s2 in
+        if start_with ";" s3 is Some n3 then
+          (ascii_of_nat v) :: html_unescape (drop n3 s3)
+        else
+          "&"%char :: html_unescape s1
+      else if sindex ";"%char s1 is Some n1 then
+        let name := take n1 s1 in
+        let s2 := drop n1 s1 in
+        if start_with ";" s2 is Some n2 then
+          let s3 := drop n2 s2 in
+          if rassoc name html_char_entities is Some (c, _) then
+            c :: html_unescape s3
+          else
+            "&"%char :: html_unescape s1
+        else
+          "&"%char :: html_unescape s1
+      else
+        "&"%char :: html_unescape s1
+  | c :: s1 => c :: html_unescape s1
+  end.
+
+(* pointer to byte (unsigned char).
+  "cptr i lst" represents a pointer to i'th char in lst.
+  restriction: 0 <= i <= size lst.
+  Although a pointer with i = size lst is valid, its dereference is invalid.
+*)
+Inductive byteptr := bptr : nat -> seq ascii -> byteptr.
+
+(* accessors for Coq proof *)
+Definition i_of_bptr ptr := let: bptr i s := ptr in i.
+Definition s_of_bptr ptr := let: bptr i s := ptr in s.
+
+(* precondition: i + n <= size s
+  C: p + n *)
+Definition bptradd ptr n :=
+  let i := i_of_bptr ptr in
+  let s := s_of_bptr ptr in
+  bptr (i + n) s.
+
+(* precondition: n <= i
+  C: p - n *)
+Definition bptrsub ptr n :=
+  let i := i_of_bptr ptr in
+  let s := s_of_bptr ptr in
+  bptr (i - n) s.
+
+(* precondition: i < size s
+  C: *p *)
+Definition bptrget ptr :=
+  let i := i_of_bptr ptr in
+  let s := s_of_bptr ptr in
+  nth "000"%char s i.
+
+(* buffer implemented using Ruby String.
+  Encoding is not considiered.
+  The C type is struct rbuf { size_t len; VALUE str }.
+  "len" is used to detect the non-linear use of the string.
+  If the string is used linearly, len == RSTRING_LEN(str) is hold.
+  We assume this condition in following explanation.
+ *)
+Inductive buffer := bufctr of seq ascii.
+
+(* accessor for Coq proof *)
+Definition s_of_buf buf := let: bufctr s := buf in s.
+
+(* (struct rbuf){ len + 1, rb_str_buf_cat(str, &b, 1) } *)
+Definition bufaddbyte buf b :=
+  let s := s_of_buf buf in
+  bufctr (rcons s b).
+
+(* precondition: i + n <= size s'
+  (struct rbuf){ len + n, rb_str_buf_cat(str, ptr, n) }
+ *)
+Definition bufaddmem buf ptr n :=
+  let s := s_of_buf buf in
+  let i := i_of_bptr ptr in
+  let s' := s_of_bptr ptr in
+  bufctr (s ++ take n (drop i s')).
+
+(* This function will be implemented as a table in C *)
+Definition html_escape_byte_table c :=
+  if assoc c html_escape_alist is Some p then
+    let s := "&" ++ p.2 ++ ";" in
+    (bptr 0 s, size s)
+  else
+    (bptr 0 [:: c], 1).
+
+Fixpoint trec_html_escape buf ptr n :=
+  match n with
+  | 0 => buf
+  | n'.+1 =>
+      let: (escptr, escn) := html_escape_byte_table (bptrget ptr) in
+      trec_html_escape
+        (bufaddmem buf escptr escn)
+        (bptradd ptr 1)
+        n'
+  end.
+
+Definition trec_html_escape_stub s :=
+  s_of_buf (trec_html_escape (bufctr [::]) (bptr 0 s) (size s)).
+
+Inductive m128 := c128 :
+  ascii -> ascii -> ascii -> ascii ->
+  ascii -> ascii -> ascii -> ascii ->
+  ascii -> ascii -> ascii -> ascii ->
+  ascii -> ascii -> ascii -> ascii -> m128.
+
+Definition seq_of_m128 m :=
+  let: c128 b0 b1 b2 b3 b4 b5 b6 b7 b8 b9 ba bb bc bd be bf := m in
+  [:: b0; b1; b2; b3; b4; b5; b6; b7; b8; b9; ba; bb; bc; bd; be; bf].
+
+Definition m128_of_seq s := c128
+  (nth "000"%char s 0) (nth "000"%char s 1) (nth "000"%char s 2) (nth "000"%char s 3)
+  (nth "000"%char s 4) (nth "000"%char s 5) (nth "000"%char s 6) (nth "000"%char s 7)
+  (nth "000"%char s 8) (nth "000"%char s 9) (nth "000"%char s 10) (nth "000"%char s 11)
+  (nth "000"%char s 12) (nth "000"%char s 13) (nth "000"%char s 14) (nth "000"%char s 15).
+
+Definition m128_of_bptr ptr := m128_of_seq (drop (i_of_bptr ptr) (s_of_bptr ptr)).
+
+(* _mm_cmpestri(a, la, b, lb,
+     _SIDD_UBYTE_OPS|_SIDD_CMP_EQUAL_ANY|
+     _SIDD_POSITIVE_POLARITY|_SIDD_LEAST_SIGNIFICANT) *)
+Definition cmpestri_ubyte_eqany_ppol_lsig (a : m128) (la : nat) (b : m128) (lb : nat) :=
+  let sa := take la (seq_of_m128 a) in
+  let sb := take lb (seq_of_m128 b) in
+  let p := mem sa in
+  if has p sb then find p sb else 16.
+
+Definition chars_to_escape_list := [:: "&"%char; "<"%char; ">"%char; """"%char; "'"%char].
+Definition chars_to_escape := m128_of_seq chars_to_escape_list.
+Definition num_chars_to_escape := size chars_to_escape_list.
+
+Fixpoint sse_html_escape buf ptr m n :=
+  match n with
+  | 0 => bufaddmem buf ptr m
+  | n'.+1 =>
+      let p1 := bptradd ptr m in
+      if n <= 15 then
+        trec_html_escape (bufaddmem buf ptr m) p1 n
+      else
+        let i := cmpestri_ubyte_eqany_ppol_lsig
+            chars_to_escape num_chars_to_escape
+            (m128_of_bptr p1) 16 in
+        if 16 <= i then
+          sse_html_escape buf ptr (m + 16) (n' - 15)
+        else
+          let buf2 := bufaddmem buf ptr (m + i) in
+          let p2 := bptradd ptr (m + i) in
+          let c := bptrget p2 in
+          let p3 := bptradd p2 1 in
+          let: (escptr, escn) := html_escape_byte_table c in
+          let buf3 := bufaddmem buf2 escptr escn in
+          sse_html_escape buf3 p3 0 (n' - i)
+  end.
+
+Definition sse_html_escape_stub s :=
+  s_of_buf (sse_html_escape (bufctr [::]) (bptr 0 s) 0 (size s)).
