coq/theories/spec.v
@@ -1,0 +1,36 @@
+From mathcomp Require Import all_ssreflect.
+Require Import String.
+Require Import Ascii.
+
+Require Import htmlescape.listutils.
+Require Import htmlescape.assoc.
+Require Import htmlescape.ssrstr.
+
+Definition html_char_entities :=
+  map (fun p => (p.1, seq_of_str p.2)) [::
+  ("&"%char, "amp");
+  ("<"%char, "lt");
+  (">"%char, "gt");
+  (""""%char, "quot");
+  ("'"%char, "apos")
+  (* ... more character entities here ... *)
+].
+
+(* HTML character and text specification.
+ * https://html.spec.whatwg.org/multipage/syntax.html#text-2
+ * Note: Unicode is not considered.
+ *)
+Inductive char_spec : ascii -> seq ascii -> Prop :=
+  | char_normal : forall c, c != "&"%char -> char_spec c [:: c]
+  | char_named : forall c entity, (c, entity) \in html_char_entities ->
+      char_spec c ("&" ++ entity ++ ";")
+  | char_dec : forall m digs, digs != nil -> decode_decimal digs = Some m ->
+      char_spec (ascii_of_nat m) ("&#" ++ digs ++ ";")
+  | char_hex : forall x m xdigs,
+      downcase_ascii x == "x"%char -> xdigs != nil -> decode_hex xdigs = Some m ->
+      char_spec (ascii_of_nat m) ("&#" ++ x :: xdigs ++ ";").
+
+Inductive text_spec : seq ascii -> seq ascii -> Prop :=
+  | text_empty : text_spec [::] [::]
+  | text_cons : forall c s raw escaped,
+      char_spec c s -> text_spec raw escaped -> text_spec (c :: raw) (s ++ escaped).
